Update to compcert-3.9 with external flocq (3.4.2)

theories/compcert/common/Sections.mli
@@ -1,0 +1,58 @@
+(* *********************************************************************)
+(*                                                                     *)
+(*              The Compcert verified compiler                         *)
+(*                                                                     *)
+(*          Xavier Leroy, INRIA Paris-Rocquencourt                     *)
+(*                                                                     *)
+(*  Copyright Institut National de Recherche en Informatique et en     *)
+(*  Automatique.  All rights reserved.  This file is distributed       *)
+(*  under the terms of the GNU Lesser General Public License as        *)
+(*  published by the Free Software Foundation, either version 2.1 of   *)
+(*  the License, or  (at your option) any later version.               *)
+(*  This file is also distributed under the terms of the               *)
+(*  INRIA Non-Commercial License Agreement.                            *)
+(*                                                                     *)
+(* *********************************************************************)
+
+
+(* Handling of linker sections *)
+
+type initialized =
+  | Uninit       (* uninitialized data area *)
+  | Init         (* initialized with fixed, non-relocatable data *)
+  | Init_reloc   (* initialized with relocatable data (symbol addresses) *)
+
+type section_name =
+  | Section_text
+  | Section_data of initialized
+  | Section_small_data of initialized
+  | Section_const of initialized
+  | Section_small_const of initialized
+  | Section_string
+  | Section_literal
+  | Section_jumptable
+  | Section_user of string * bool (*writable*) * bool (*executable*)
+  | Section_debug_abbrev
+  | Section_debug_info of string option
+  | Section_debug_loc
+  | Section_debug_line of string option
+  | Section_debug_ranges
+  | Section_debug_str
+  | Section_ais_annotation
+
+type access_mode =
+  | Access_default
+  | Access_near
+  | Access_far
+
+val initialize: unit -> unit
+
+val define_section:
+  string -> ?iname:string -> ?uname:string
+         -> ?writable:bool -> ?executable:bool -> ?access:access_mode -> unit -> unit
+val use_section_for: AST.ident -> string -> bool
+
+val for_variable: Env.t -> C.location -> AST.ident -> C.typ -> initialized ->
+                                          section_name * access_mode
+val for_function: Env.t -> C.location -> AST.ident -> C.attributes -> section_name list
+val for_stringlit: unit -> section_name
