theories/compcert/common/Unityping.v
@@ -6,17 +6,17 @@
 (*                                                                     *)
 (*  Copyright Institut National de Recherche en Informatique et en     *)
 (*  Automatique.  All rights reserved.  This file is distributed       *)
-(*  under the terms of the GNU General Public License as published by  *)
-(*  the Free Software Foundation, either version 2 of the License, or  *)
-(*  (at your option) any later version.  This file is also distributed *)
-(*  under the terms of the INRIA Non-Commercial License Agreement.     *)
+(*  under the terms of the GNU Lesser General Public License as        *)
+(*  published by the Free Software Foundation, either version 2.1 of   *)
+(*  the License, or  (at your option) any later version.               *)
+(*  This file is also distributed under the terms of the               *)
+(*  INRIA Non-Commercial License Agreement.                            *)
 (*                                                                     *)
 (* *********************************************************************)
 
 (* A solver for unification constraints. *)
 
 Require Import Recdef Coqlib Maps Errors.
-Require Import Coq.micromega.Lia.
 
 Local Open Scope nat_scope.
 Local Open Scope error_monad_scope.
@@ -200,7 +200,7 @@ Proof.
   apply A. rewrite PTree.gso by congruence. auto.
 Qed.
 
-Hint Resolve set_incr: ty.
+Global Hint Resolve set_incr: ty.
 
 Lemma set_sound:
   forall te x ty e e', set e x ty = OK e' -> satisf te e' -> te x = ty.
@@ -217,7 +217,7 @@ Proof.
   induction xl; destruct tyl; simpl; intros; monadInv H; eauto with ty.
 Qed.
 
-Hint Resolve set_list_incr: ty.
+Global Hint Resolve set_list_incr: ty.
 
 Lemma set_list_sound:
   forall te xl tyl e e', set_list e xl tyl = OK e' -> satisf te e' -> map te xl = tyl.
@@ -243,7 +243,7 @@ Proof.
 - inv H; simpl in *; split; auto.
 Qed.
 
-Hint Resolve move_incr: ty.
+Global Hint Resolve move_incr: ty.
 
 Lemma move_sound:
   forall te e r1 r2 e' changed,
